%!TEX TS-program = xelatex
%!TEX options = -aux-directory=Debug -shell-escape -file-line-error -interaction=nonstopmode -halt-on-error -synctex=1 "%DOC%"
\documentclass{article}
\input{LaTeX-Submodule/template.tex}

% Additional packages & macros
\theoremstyle{definition}
\newtheorem{example}{Example}[section]

% Header and footer
\newcommand{\unitName}{Differential Equations and Modelling 2}
\newcommand{\unitTime}{Semester 2, 2024}
\newcommand{\unitCoordinator}{Professor Scott McCue}
\newcommand{\documentAuthors}{Tarang Janawalkar}

\fancyhead[L]{\unitName}
\fancyhead[R]{\leftmark}
\fancyfoot[C]{\thepage}

% Copyright
\usepackage[
    type={CC},
    modifier={by-nc-sa},
    version={4.0},
    imagewidth={5em},
    hyphenation={raggedright}
]{doclicense}

\date{}

\begin{document}
%
\begin{titlepage}
    \vspace*{\fill}
    \begin{center}
        \LARGE{\textbf{\unitName}} \\[0.1in]
        \normalsize{\unitTime} \\[0.2in]
        \normalsize\textit{\unitCoordinator} \\[0.2in]
        \documentAuthors
    \end{center}
    \vspace*{\fill}
    \doclicenseThis
    \thispagestyle{empty}
\end{titlepage}
\newpage
%
\tableofcontents
\newpage
%
\part{Symmetry Methods}
\section{Symmetry Transformations}
Consider a partial differential equation for \(u\left( x,\: t \right)\)
whose domain lies in \(\R^2\). Such a problem typically does not have
any natural length or time scales associated with it's fundamental
solution. Thus, let us transform the independent and dependent
variables through the mapping \(\left( x,\: t,\: u \right) \mapsto
\left( X,\: T,\: U \right)\) where \(X = X\left( x,\: t,\: u \right)\),
\(T = T\left( x,\: t,\: u \right)\), and \(U = U\left( x,\: t,\: u
\right)\), such that the PDE is invariant under this transformation,
that is, the transformed PDE in \(U\) has the same form as the original
PDE in \(u\).

The choice of mapping may consist of dilations and translations of the
independent and dependent variables by some constant factors, where
each constant is enforced by the invariance condition. To do this, we
must ensure that the function \(U\left( x,\: t,\: u\left( X,\: T
\right) \right)\) satisfies the transformed PDE. When this is the case,
the PDE is said to have a \textit{symmetry transformation}.

The goal of these symmetry methods is to find an appropriate
transformation that simplies the PDE, often reducing it to an ODE.
\subsection{Dilation Symmetry}
A dilation symmetry is a transformation of the form
\begin{equation*}
    X = a x, \quad T = a^\beta t, \quad U = a^\gamma u,
\end{equation*}
where \(a\), \(\beta\), and \(\gamma\) are constants. Note that we do
not express the transformation for \(x\) as \(X = a^\alpha x\) since it
does not provide any additional information.
\begin{example}
    Consider the transport equation
    \begin{equation*}
        \pdv{u\left( x,\: t \right)}{t} + c \pdv{u\left( x,\: t \right)}{x} = 0
    \end{equation*}
    and the mapping
    \begin{equation*}
        X = a x, \quad T = a^\beta t, \quad U = u.
    \end{equation*}
    After substituting the transformed solution into the PDE, we find
    \begin{align*}
        \pdv{u\left( X,\: T \right)}{t} + c \pdv{u\left( X,\: T \right)}{x}                       & = 0  \\
        \pdv{u\left( X,\: T \right)}{T} \odv{T}{t} + c \pdv{u\left( X,\: T \right)}{X} \odv{X}{x} & = 0  \\
        a^\beta \pdv{u\left( X,\: T \right)}{T} + a c \pdv{u\left( X,\: T \right)}{X}             & = 0.
    \end{align*}
    For this PDE to be invariant under a dilation transformation, we
    must factor out the constant \(a\) from the equation. This implies
    that:
    \begin{equation*}
        a^\beta = a \implies \beta = 1,
    \end{equation*}
    so that
    \begin{equation*}
        \pdv{u\left( X,\: T \right)}{T} + c \pdv{u\left( X,\: T \right)}{X} = 0.
    \end{equation*}
    Here we have shown that the transport equation is invariant under
    the above dilation transformation when \(\beta = 1\).
\end{example}
\begin{example}
    Consider the nonlinear PDE
    \begin{equation*}
        \pdv{u\left( x,\: y \right)}{x} + y^2 \pdv{u\left( x,\: y \right)}{y} = 0
    \end{equation*}
    and the mapping
    \begin{equation*}
        X = a x, \quad Y = a^\beta y, \quad U = u.
    \end{equation*}
    By substituting the transformed solution into the PDE, we find
    \begin{align*}
        \pdv{u\left( X,\: Y \right)}{x} + y^2 \pdv{u\left( X,\: Y \right)}{y}                                    & = 0  \\
        \pdv{u\left( X,\: Y \right)}{X} \odv{X}{x} + y^2 \pdv{u\left( X,\: Y \right)}{Y} \odv{Y}{y}              & = 0  \\
        a \pdv{u\left( X,\: Y \right)}{X} + a^\beta y^2 \pdv{u\left( X,\: Y \right)}{Y}                          & = 0  \\
        a \pdv{u\left( X,\: Y \right)}{X} + a^\beta \left( Y / a^\beta \right)^2 \pdv{u\left( X,\: Y \right)}{Y} & = 0  \\
        a \pdv{u\left( X,\: Y \right)}{X} + a^{-\beta} Y^2 \pdv{u\left( X,\: Y \right)}{Y}                       & = 0.
    \end{align*}
    For this PDE to be invariant under a dilation transformation, we
    must again factor out \(a\) from the equation so that:
    \begin{equation*}
        a = a^{-\beta} \implies 1 = -\beta \implies \beta = -1,
    \end{equation*}
    and
    \begin{equation*}
        \pdv{u\left( X,\: Y \right)}{X} + Y^2 \pdv{u\left( X,\: Y \right)}{Y} = 0.
    \end{equation*}
    Here we have shown that this nonlinear PDE is invariant under the
    above dilation transformation when \(\beta = -1\).
\end{example}
\begin{example}
    Consider the nonlinear convection diffusion equation
    \begin{equation*}
        \pdv{u\left( x,\: t \right)}{t} = u\left( x,\: t \right) \pdv[order=2]{u\left( x,\: t \right)}{x} - \pdv{u\left( x,\: t \right)}{x}
    \end{equation*}
    and the mapping
    \begin{equation*}
        X = a x, \quad T = a^\beta t, \quad U = a^\gamma u.
    \end{equation*}
    We will once again substitute the transformed solution into the PDE
    to find
    \begin{align*}
        a^\gamma \pdv{u\left( X,\: T \right)}{t}            & = a^{2\gamma} u\left( X,\: T \right) \pdv[order=2]{u\left( X,\: T \right)}{x} - a^\gamma \pdv{u\left( X,\: T \right)}{x}                                       \\
        a^\gamma \pdv{u\left( X,\: T \right)}{T} \odv{T}{t} & = a^{2\gamma} u\left( X,\: T \right) \pdv*{\left[ \pdv{u\left( X,\: T \right)}{X} \odv{X}{x} \right]}{x} - a^\gamma \pdv{u\left( X,\: T \right)}{X} \odv{X}{x} \\
        a^{\beta + \gamma} \pdv{u\left( X,\: T \right)}{T}  & = a^{1 + 2\gamma} u\left( X,\: T \right) \pdv*{\left[ \odv{X}{x} \pdv{u\left( X,\: T \right)}{X} \right]}{X} - a^{1 + \gamma} \pdv{u\left( X,\: T \right)}{X}  \\
        a^{\beta + \gamma} \pdv{u\left( X,\: T \right)}{T}  & = a^{2 + 2\gamma} u\left( X,\: T \right) \pdv[order=2]{u\left( X,\: T \right)}{X} - a^{1 + \gamma} \pdv{u\left( X,\: T \right)}{X}.
    \end{align*}
    For this PDE to be invariant under a dilation transformation, we
    must factor out \(a\) from the equation so that:
    \begin{equation*}
        a^{\beta + \gamma} = a^{2 + 2\gamma} = a^{1 + \gamma} \implies \beta + \gamma = 2 + 2\gamma = 1 + \gamma \implies \beta = 1, \gamma = -1,
    \end{equation*}
    and
    \begin{equation*}
        \pdv{u\left( X,\: T \right)}{T} = u\left( X,\: T \right) \pdv[order=2]{u\left( X,\: T \right)}{X} - \pdv{u\left( X,\: T \right)}{X}.
    \end{equation*}
    Here we have shown that this nonlinear PDE is invariant under the
    above dilation transformation when \(\beta = 1\) and \(\gamma = -1\).
\end{example}
\subsection{Translation Symmetry}
A translation symmetry is a transformation of the form
\begin{equation*}
    X = x - x_0, \quad T = t - t_0, \quad U = u - u_0,
\end{equation*}
where \(x_0\), \(t_0\), and \(u_0\) are constants.
\begin{example}
    Consider the heat equation
    \begin{equation*}
        \pdv{u\left( x,\: t \right)}{t} = D \pdv[order=2]{u\left( x,\: t \right)}{x}
    \end{equation*}
    and the mapping
    \begin{equation*}
        X = x - x_0, \quad T = t - t_0, \quad U = u - u_0.
    \end{equation*}
    By substituting the transformed solution into the PDE, we find
    \begin{align*}
        \pdv*{\left( u\left( X,\: T \right) - u_0 \right)}{t} & = D \pdv*[order=2]{\left( u\left( X,\: T \right) - u_0 \right)}{x}      \\
        \pdv{u\left( X,\: T \right)}{T} \odv{T}{t}            & = D \pdv*{\left( \pdv{u\left( X,\: T \right)}{X} \odv{X}{x} \right)}{x} \\
        \pdv{u\left( X,\: T \right)}{T}                       & = D \pdv{}{X} \odv{X}{x} \left( \pdv{u\left( X,\: T \right)}{X} \right) \\
        \pdv{u\left( X,\: T \right)}{T}                       & = D \pdv[order=2]{u\left( X,\: T \right)}{X}.
    \end{align*}
    Here we have shown that the heat equation is invariant under the
    above translation transformation.
\end{example}
\section{Similarity Solutions}
In the previous section, we considered dilation transformations where
both independent variables were scaled by some power of \(a\). Notice
that the product \(\eta = x t^{-1/\beta}\) is invariant under the same
dilation transformation:
\begin{align*}
    \eta = x t^{-1/\beta} \implies H = \left( \frac{x}{a} \right) \left( \frac{T}{a^\beta} \right)^{-1/\beta} = X T^{-1/\beta}.
\end{align*}
Let us therefore consider transformations of the form
\begin{equation*}
    X = a x, \quad T = a^\beta t, \quad U = t^{-\alpha} f\left( \eta \right),
\end{equation*}
where \(a\), \(\alpha\), and \(\beta\) are constant and \(f\) is an arbitrary
function to be determined. \(f\) is called a \textit{similarity solution}
(with \textit{similarity variable} \(\eta\)) and our goal is to
transform the PDE into an ODE with a single independent variable \(\eta\).
To do this:
\begin{enumerate}
    \item Substitute \(u\left( X,\: T \right)\) into the PDE to solve
          for \(\alpha\) and \(\beta\) while maintaining invariance.
    \item Obtain an ODE in terms of \(f\left( \eta \right)\) by
          substituting the similarity solution into the PDE.
    \item Obtain boundary conditions in terms of \(\eta\) using the
          same transformation.
    \item Solve the ODE to find \(f\left( \eta \right)\).
    \item Transform back to the original variables to find a solution
          to the PDE.
\end{enumerate}
\section{Travelling Wave Solutions}
Another type of solution is the \textit{travelling wave solution},
where the solution to a PDE appears to move at a constant velocity when
after a long period of time. This is similar to a steady state solution
where the solution does not change after a long period of time. In this
problem, we assume solutions of the form
\begin{equation*}
    u\left( x,\: t \right) = f\left( z \right), \quad z = x - c t,
\end{equation*}
where \(c\) is the speed at which the solution travels. The travelling
wave speed is often determined using analysis, boundary conditions,
numerical methods, or physical constraints. This method is only
applicable to PDEs that are invariant under translations to both
independent variables. As such, the PDE must not contain any explicit
dependence on \(x\) or \(t\).
\part{Method of Characteristics}
The method of characteristics is a technique used to solve nonlinear
PDEs by reducing them to a system of ODEs. It considers
parametrisations of the solution through a set of curves in the
solution space.
\section{First Order PDEs}
\subsection{Classification}
Consider the general first order PDE in two variables:
\begin{equation*}
    a \pdv{u}{x} + b \pdv{u}{y} = f.
\end{equation*}
We can classify this PDE into 3 types based on the value of the
variables \(a\), \(b\), and \(f\):
\begin{itemize}
    \item \textbf{Linear}:
          \begin{equation*}
              a\left( x,\: y \right) \pdv{u}{x} + b\left( x,\: y \right) \pdv{u}{y} = f\left( x,\: y \right).
          \end{equation*}
    \item \textbf{Semi-Linear}:
          \begin{equation*}
              a\left( x,\: y \right) \pdv{u}{x} + b\left( x,\: y \right) \pdv{u}{y} = f\left( x,\: y,\: u \right).
          \end{equation*}
    \item \textbf{Quasi-Linear}:
          \begin{equation*}
              a\left( x,\: y,\: u \right) \pdv{u}{x} + b\left( x,\: y,\: u \right) \pdv{u}{y} = f\left( x,\: y,\: u \right).
          \end{equation*}
    \item \textbf{Nonlinear}: Otherwise.
\end{itemize}
\subsection{Characteristics}
Given a quasi-linear PDE of the form:
\begin{equation*}
    a\left( x,\: y,\: u \right) \pdv{u}{x} + b\left( x,\: y,\: u \right) \pdv{u}{y} = f\left( x,\: y,\: u \right)
\end{equation*}
with the initial condition \(u\left( x,\: 0 \right) = u_0\left( x \right)\),
let us consider the surface \(u = u\left( x,\: y \right)\), which has
the normal vector:
\begin{equation*}
    \symbf{n} =
    \begin{bmatrix}
        \pdv{u}{x} \\
        \pdv{u}{y} \\
        -1
    \end{bmatrix}
    .
\end{equation*}
We can find a tangent vector to \(\symbf{n}\) by using the orthogonality
property of the dot product of the normal vector:
\begin{equation*}
    \begin{bmatrix}
        a\left( x,\: y,\: u \right) \\
        b\left( x,\: y,\: u \right) \\
        f\left( x,\: y,\: u \right)
    \end{bmatrix}
    \cdot
    \symbf{n}
    = 0,
\end{equation*}
Let us call this vector \(\symbf{v}\):
\begin{equation*}
    \symbf{v} =
    \begin{bmatrix}
        a\left( x,\: y,\: u \right) \\
        b\left( x,\: y,\: u \right) \\
        f\left( x,\: y,\: u \right)
    \end{bmatrix}
    .
\end{equation*}
Let us now consider a parametric curve defined:
\begin{equation*}
    \symbf{r}\left( s \right) =
    \begin{bmatrix}
        x\left( s \right) \\
        y\left( s \right) \\
        u\left( s \right)
    \end{bmatrix}
\end{equation*}
and let us impose that \(\symbf{r}'\left( s \right) = \symbf{v}\), so
that the curve lies on the solution surface. This gives us the following
system of equations:
\begin{equation*}
    \symbf{r}'\left( s \right) = \symbf{v} \iff
    \begin{cases}
        \displaystyle\pdv{x}{s} = a\left( x,\: y,\: u \right), \\
        \displaystyle\pdv{y}{s} = b\left( x,\: y,\: u \right), \\
        \displaystyle\pdv{u}{s} = f\left( x,\: y,\: u \right).
    \end{cases}
\end{equation*}
These equations are called \textit{characteristic curves} of the PDE.
We can integrate each of these equations to find parametric curves in
\(s\), and solve for all integration constants using the initial
condition:
\begin{equation*}
    u\left( 0 \right) = u_0\left( \xi \right).
\end{equation*}
where \(x = \xi\)\footnote{\(\xi\) is introduced to avoid
    confusion with the variable \(x\) in the initial condition.}
and \(y = 0\). We can
then solve for \(u\left( x,\: y \right)\) by eliminating \(s\) and
\(\xi\) from the parametric equations.
\end{document}
